fix common/ast.v and all uses

coq/common/ast.v
@@ -1,139 +1,104 @@
 Require Import CAS.coq.common.compute.
 
-Inductive cas_ast : Type :=
-   | Ast_eqv_bool          : cas_ast
-   | Ast_eqv_nat           : cas_ast
-   | Ast_eqv_list          : cas_ast → cas_ast
-   | Ast_eqv_set           : cas_ast → cas_ast
-   | Ast_eqv_product       : cas_ast * cas_ast → cas_ast
-   | Ast_eqv_sum           : cas_ast * cas_ast → cas_ast
-   | Ast_eqv_add_constant  : cas_constant * cas_ast → cas_ast
-   | Ast_eqv_nat_ceiling   : nat → cas_ast   
-   | Ast_eqv_minset        : cas_ast → cas_ast
-
-   | Ast_po_subset        : cas_ast → cas_ast
-   | Ast_po_dual          : cas_ast → cas_ast
-   | Ast_po_product       : cas_ast * cas_ast → cas_ast
-   | Ast_po_left_sum      : cas_ast * cas_ast → cas_ast
-   | Ast_po_right_sum     : cas_ast * cas_ast → cas_ast
-   | Ast_po_add_bottom    : cas_constant * cas_ast → cas_ast
-   | Ast_po_add_top       : cas_constant * cas_ast → cas_ast
-   | Ast_po_from_qo       : cas_ast → cas_ast
-   | Ast_po_from_to       : cas_ast → cas_ast
-   | Ast_po_llte          : cas_ast → cas_ast
-   | Ast_po_rlte          : cas_ast → cas_ast
-   | Ast_qo_trivial       : cas_ast → cas_ast
-   | Ast_qo_length        : cas_ast → cas_ast                                                                                   
-
-   | Ast_to_nat           : cas_ast
-   | Ast_to_bool          : cas_ast
-   | Ast_to_from_po       : cas_ast → cas_ast
-   | Ast_to_llte          : cas_ast → cas_ast
-   | Ast_to_rlte          : cas_ast → cas_ast
-
-   | Ast_sg_times        : cas_ast
-   | Ast_sg_plus         : cas_ast
-   | Ast_sg_and          : cas_ast 
-   | Ast_sg_or           : cas_ast 
-   | Ast_sg_min          : cas_ast 
-   | Ast_sg_max          : cas_ast
-   | Ast_sg_union        : cas_ast → cas_ast
-   | Ast_sg_intersect    : cas_ast → cas_ast                             
-   | Ast_sg_concat       : cas_ast → cas_ast                                
-   | Ast_sg_left         : cas_ast → cas_ast
-   | Ast_sg_right        : cas_ast → cas_ast
-
-   | Ast_sg_product        : cas_ast * cas_ast → cas_ast
-   | Ast_sg_llex           : cas_ast * cas_ast → cas_ast
-   | Ast_sg_add_id         : cas_constant * cas_ast → cas_ast
-   | Ast_sg_add_ann        : cas_constant * cas_ast → cas_ast                                                   
-   | Ast_sg_left_sum       : cas_ast * cas_ast → cas_ast
-   | Ast_sg_right_sum      : cas_ast * cas_ast → cas_ast
-   | Ast_sg_lift           : cas_ast → cas_ast      
-   | Ast_sg_minset_union   : cas_ast → cas_ast                                                
-   | Ast_sg_minset_lift    : cas_ast → cas_ast                                          
-
-   | Ast_sg_from_sg_C      : cas_ast → cas_ast                                                
-   | Ast_sg_C_from_sg_CI   : cas_ast → cas_ast
-   | Ast_sg_C_from_sg_CK   : cas_ast → cas_ast
-   | Ast_sg_C_from_sg      : cas_ast → cas_ast
-   | Ast_sg_CK_from_sg     : cas_ast → cas_ast
-   | Ast_sg_CK_from_sg_C   : cas_ast → cas_ast
-   | Ast_sg_CI_from_sg_CS  : cas_ast → cas_ast
-   | Ast_sg_CI_from_sg_C   : cas_ast → cas_ast
-   | Ast_sg_CS_from_sg_CI  : cas_ast → cas_ast
-   | Ast_sg_CS_from_sg_C   : cas_ast → cas_ast                             
-   | Ast_asg_from_sg        : cas_ast → cas_ast
-   | Ast_msg_from_sg        : cas_ast → cas_ast 
-
-
-   | Ast_min_plus : cas_ast
-   | Ast_max_plus : cas_ast
-   | Ast_and_or   : cas_ast                                                                           
-   | Ast_union_intersect : cas_ast → cas_ast
-   | Ast_max_min   : cas_ast
-   | Ast_min_max   : cas_ast
-                                        
-   | Ast_bs_product    : cas_ast * cas_ast → cas_ast
-   | Ast_bs_left_sum   : cas_ast * cas_ast → cas_ast
-   | Ast_bs_right_sum  : cas_ast * cas_ast → cas_ast     
-   | Ast_bs_add_zero   : cas_constant * cas_ast → cas_ast
-   | Ast_bs_add_one    : cas_constant * cas_ast → cas_ast
-   | Ast_bs_llex       : cas_ast * cas_ast → cas_ast                                                   
-   | Ast_bs_union_lift : cas_ast → cas_ast
-   | Ast_bs_dual : cas_ast → cas_ast                                     
-
-   | Ast_bs_CI_from_bs       : cas_ast → cas_ast
-   | Ast_bs_CI_from_bs_CS    : cas_ast → cas_ast                                          
-   | Ast_bs_CI_from_lattice  : cas_ast → cas_ast                                       
-   | Ast_bs_CS_from_bs_CI   : cas_ast  → cas_ast
-   | Ast_bs_CS_from_bs      : cas_ast  → cas_ast                                       
-   | Ast_bs_from_bs_CI       : cas_ast → cas_ast                                       
-   | Ast_bs_from_presemiring : cas_ast → cas_ast
-
-   | Ast_presemiring_product     : cas_ast * cas_ast → cas_ast
-   | Ast_mposg_from_bs                    : cas_ast → cas_ast                                            
-   | Ast_presemiring_from_bs                    : cas_ast → cas_ast                                                                      
-   | Ast_presemiring_from_semiring              : cas_ast → cas_ast
-| Ast_presemiring_from_selective_presemiring : cas_ast → cas_ast
-| Ast_presemiring_from_distributive_prelattice : cas_ast → cas_ast
-| Ast_presemiring_from_selective_distributive_prelattice : cas_ast → cas_ast                                          
-| Ast_selective_presemiring_from_presemiring  : cas_ast → cas_ast                                                            
-| Ast_semiring_from_presemiring  : cas_ast → cas_ast                                                            
-| Ast_semiring_from_dioid        : cas_ast → cas_ast
-| Ast_semiring_from_selective_semiring  : cas_ast → cas_ast 
-| Ast_selective_semiring_from_semiring  : cas_ast → cas_ast                                                            
-| Ast_dioid_from_semiring             : cas_ast → cas_ast                                        
-| Ast_dioid_from_distributive_lattice : cas_ast → cas_ast
-| Ast_dioid_from_selective_dioid      : cas_ast → cas_ast
-| Ast_selective_dioid_from_dioid                           : cas_ast → cas_ast
-| Ast_selective_dioid_from_selective_distributive_lattice  : cas_ast → cas_ast                                       
-| Ast_distributive_lattice_from_dioid                           : cas_ast → cas_ast
-| Ast_distributive_lattice_from_lattice                         : cas_ast → cas_ast
-| Ast_distributive_lattice_from_selective_distributive_lattice  : cas_ast → cas_ast
-| Ast_selective_distributive_lattice_from_selective_dioid       : cas_ast → cas_ast
-| Ast_selective_distributive_lattice_from_distributive_lattice  : cas_ast → cas_ast
-  | Ast_lattice_from_bs_CI                  : cas_ast → cas_ast                                                          
-  | Ast_lattice_from_distributive_lattice   : cas_ast → cas_ast
-| Ast_distributive_prelattice_from_selective_distributive_prelattice  : cas_ast → cas_ast
-
-| Ast_po_from_sg_left : cas_ast → cas_ast
-| Ast_po_from_sg_right : cas_ast → cas_ast                              
-| Ast_os_from_bs_left : cas_ast → cas_ast
-| Ast_os_from_bs_right : cas_ast → cas_ast                                     
-
-   | Ast_ltr_cons          : cas_ast            → cas_ast    
-   | Ast_ltr_right         : cas_ast * cas_ast  → cas_ast
-   | Ast_ltr_product       : cas_ast * cas_ast  → cas_ast
-   | Ast_ltr_left_sum      : cas_ast * cas_ast  → cas_ast
-   | Ast_ltr_right_sum     : cas_ast * cas_ast  → cas_ast
-   | Ast_ltr_lift          : cas_ast            → cas_ast
-   | Ast_ltr_lift_all      : cas_ast            → cas_ast
-   | Ast_ltr_with_policy   : cas_ast            → cas_ast                                                     
-   | Ast_ltr_from_sg       : cas_ast             → cas_ast
-   | Ast_ltr_from_sg_C     : cas_ast           → cas_ast
-   | Ast_ltr_from_sg_CI    : cas_ast          → cas_ast
-   | Ast_ltr_from_sg_CS    : cas_ast          → cas_ast
-   | Ast_ltr_from_sg_CK    : cas_ast          → cas_ast   
-
+  
+Inductive cas_eqv_ast : Type :=
+   | Ast_eqv_bool          : cas_eqv_ast
+   | Ast_eqv_nat           : cas_eqv_ast
+   | Ast_eqv_list          : cas_eqv_ast → cas_eqv_ast
+   | Ast_eqv_set           : cas_eqv_ast → cas_eqv_ast
+   | Ast_eqv_product       : cas_eqv_ast * cas_eqv_ast → cas_eqv_ast
+   | Ast_eqv_sum           : cas_eqv_ast * cas_eqv_ast → cas_eqv_ast
+   | Ast_eqv_add_constant  : cas_constant * cas_eqv_ast → cas_eqv_ast
+   | Ast_eqv_nat_ceiling   : nat → cas_eqv_ast   
+   | Ast_eqv_minset        : cas_or_ast → cas_eqv_ast
+   | Ast_eqv_of_or         : cas_or_ast → cas_eqv_ast
+   | Ast_eqv_of_sg         : cas_sg_ast → cas_eqv_ast
+   | Ast_eqv_of_bs         : cas_bs_ast → cas_eqv_ast
+   | Ast_eqv_of_os         : cas_os_ast → cas_eqv_ast
+with cas_or_ast : Type :=
+   | Ast_or_nat           : cas_or_ast
+   | Ast_or_bool          : cas_or_ast
+   | Ast_or_add_bottom    : cas_constant * cas_or_ast → cas_or_ast
+   | Ast_or_add_top       : cas_constant * cas_or_ast → cas_or_ast    
+   | Ast_or_dual          : cas_or_ast → cas_or_ast      
+   | Ast_or_llte          : cas_sg_ast → cas_or_ast
+   | Ast_or_rlte          : cas_sg_ast → cas_or_ast
+   | Ast_or_length        : cas_eqv_ast → cas_or_ast
+   | Ast_or_llex          : cas_or_ast * cas_or_ast → cas_or_ast
+   | Ast_or_product       : cas_or_ast * cas_or_ast → cas_or_ast    
+   | Ast_or_subset        : cas_eqv_ast → cas_or_ast
+   | Ast_or_set           : cas_eqv_ast → cas_or_ast
+   | Ast_or_left_sum      : cas_or_ast * cas_or_ast → cas_or_ast
+   | Ast_or_right_sum     : cas_or_ast * cas_or_ast → cas_or_ast
+   | Ast_or_trivial       : cas_eqv_ast → cas_or_ast
+   | Ast_or_of_os         : cas_os_ast → cas_or_ast                                               
+with cas_sg_ast : Type :=
+   | Ast_sg_times        : cas_sg_ast
+   | Ast_sg_plus         : cas_sg_ast
+   | Ast_sg_or           : cas_sg_ast
+   | Ast_sg_and          : cas_sg_ast                              
+   | Ast_sg_min          : cas_sg_ast 
+   | Ast_sg_max          : cas_sg_ast
+   | Ast_sg_add_id       : cas_constant * cas_sg_ast → cas_sg_ast
+   | Ast_sg_add_ann      : cas_constant * cas_sg_ast → cas_sg_ast    
+   | Ast_sg_concat       : cas_eqv_ast → cas_sg_ast         
+   | Ast_sg_union        : cas_constant * cas_eqv_ast → cas_sg_ast
+   | Ast_sg_intersect    : cas_constant * cas_eqv_ast → cas_sg_ast  
+   | Ast_sg_left         : cas_eqv_ast → cas_sg_ast
+   | Ast_sg_right        : cas_eqv_ast → cas_sg_ast
+   | Ast_sg_left_sum     : cas_sg_ast * cas_sg_ast → cas_sg_ast
+   | Ast_sg_right_sum    : cas_sg_ast * cas_sg_ast → cas_sg_ast
+   | Ast_sg_lift         : cas_sg_ast → cas_sg_ast
+   | Ast_sg_llex         : cas_sg_ast * cas_sg_ast → cas_sg_ast
+   | Ast_sg_product      : cas_sg_ast * cas_sg_ast → cas_sg_ast
+   | Ast_sg_minset_lift  : cas_os_ast → cas_sg_ast   
+   | Ast_sg_minset_union : cas_or_ast → cas_sg_ast
+   | Ast_sg_plus_of_bs   : cas_bs_ast → cas_sg_ast
+   | Ast_sg_times_of_bs  : cas_bs_ast → cas_sg_ast
+   | Ast_sg_times_of_os  : cas_os_ast → cas_sg_ast
+with cas_bs_ast : Type :=
+   | Ast_min_plus : cas_bs_ast
+   | Ast_max_plus : cas_bs_ast
+   | Ast_and_or   : cas_bs_ast
+   | Ast_or_and   : cas_bs_ast                      
+   | Ast_max_min   : cas_bs_ast
+   | Ast_min_max   : cas_bs_ast                      
+   | Ast_bs_add_zero   : cas_constant * cas_bs_ast → cas_bs_ast
+   | Ast_bs_add_one    : cas_constant * cas_bs_ast → cas_bs_ast  
+   | Ast_bs_product    : cas_bs_ast * cas_bs_ast → cas_bs_ast
+   | Ast_bs_llex_product       : cas_bs_ast * cas_bs_ast → cas_bs_ast
+   | Ast_bs_union_lift : cas_sg_ast → cas_bs_ast
+   | Ast_bs_left_sum_right_sum   : cas_bs_ast * cas_bs_ast → cas_bs_ast
+   | Ast_bs_right_sum_left_sum  : cas_bs_ast * cas_bs_ast → cas_bs_ast 
+   | Ast_bs_left   : cas_sg_ast  → cas_bs_ast
+   | Ast_bs_right  : cas_sg_ast  → cas_bs_ast      
+   | Ast_union_intersect : cas_constant * cas_eqv_ast → cas_bs_ast
+   | Ast_intersect_union : cas_constant * cas_eqv_ast → cas_bs_ast    
+   | Ast_bs_dual : cas_bs_ast → cas_bs_ast   
+   | Ast_minset_lift_union : cas_os_ast → cas_bs_ast    
+   | Ast_minset_union_lift : cas_os_ast → cas_bs_ast
+   | Ast_lift_union : cas_sg_ast → cas_bs_ast    
+   | Ast_union_lift : cas_sg_ast → cas_bs_ast                          
+with cas_os_ast : Type :=
+   | Ast_os_from_bs_left : cas_bs_ast  → cas_os_ast
+   | Ast_os_from_bs_right : cas_bs_ast  → cas_os_ast
+   | Ast_os_llex_product : cas_os_ast * cas_os_ast  → cas_os_ast
+   | Ast_os_product : cas_os_ast * cas_os_ast  → cas_os_ast
+   | Ast_os_add_bottom_id : cas_constant * cas_os_ast → cas_os_ast
+   | Ast_os_add_top_ann : cas_constant * cas_os_ast → cas_os_ast 
+with cas_ltr_ast : Type :=
+   | Ast_ltr_cons          : cas_eqv_ast            → cas_ltr_ast    
+   | Ast_ltr_product       : cas_ltr_ast * cas_ltr_ast  → cas_ltr_ast
+   | Ast_ltr_left_sum      : cas_ltr_ast * cas_ltr_ast  → cas_ltr_ast
+   | Ast_ltr_right_sum     : cas_ltr_ast * cas_ltr_ast  → cas_ltr_ast
+   | Ast_ltr_lift          : cas_ltr_ast            → cas_ltr_ast
+   | Ast_ltr_from_sg       : cas_ltr_ast             → cas_ltr_ast
+   | Ast_ltr_with_policy   : cas_ltr_ast            → cas_ltr_ast
+with cas_lstr_ast : Type :=
+| Ast_lstr_product         : cas_lstr_ast * cas_lstr_ast  → cas_lstr_ast
+| Ast_lstr_llex_product    : cas_lstr_ast * cas_lstr_ast  → cas_lstr_ast
+with cas_lotr_ast : Type :=
+| Ast_lotr_length_cons     : cas_eqv_ast  → cas_lotr_ast  
+| Ast_lotr_product         : cas_lotr_ast * cas_lotr_ast  → cas_lotr_ast
+| Ast_lotr_llex_product    : cas_lotr_ast * cas_lotr_ast  → cas_lotr_ast
 .
